\section{parametrisation}

	
\begin{equation}
	\left.\begin{aligned}
	{q_i}^{\mu} &= z{p_i}^{\mu} + y(1-z){p_j}^{\mu} + \sqrt{zy(1-z)}{m}_{\bot} \\
	{q}^{\mu}   &= (1-z){p_i}^{\mu} + yz {p_j}^{\mu} - \sqrt{zy(1-z)}{m}_{\bot} \\
	{q_j}^{\mu} &= (1-y) {p_j}^{\mu} \\
		y       &= \frac{q_i q}{p_i p_j} \\
q_i +q      &= p_i + yp_j \\
q_j +q      &= (1-z){p_i}^{\mu} + (1+yz-y) {p_j}^{\mu} - \sqrt{zy(1-z)}{m}_{\bot}\\
q_i \cdot q &= yz^2 (p_i \cdot p_j)+y(1-z)^2 (p_j \cdot p_i) &=y(p_i \cdot p_j)\\
q_i \cdot q_j &= z(1-y) (p_i \cdot p_j)\\
q_j \cdot q &= (1-z)(1-y) (p_i \cdot p_j)&=(1-z)(p_i \cdot p_j)
		\end{aligned}
	\right\}
	\quad \text{parametrisation}
\end{equation}

\newpage